tests/lean/run/strInterpolation.lean
@@ -12,34 +12,34 @@ c == '{' || isQuotableCharDefault c
 
 partial def strInterpolantFn (p : ParserFn) : ParserFn :=
 fun c s =>
-let input     := c.input;
-let stackSize := s.stackSize;
+let input     := c.input
+let stackSize := s.stackSize
 let rec parse (startPos : Nat) (c : ParserContext) (s : ParserState) : ParserState :=
-  let i     := s.pos;
+  let i     := s.pos
   if input.atEnd i then
     s.mkEOIError
   else
-    let curr := input.get i;
-    let s    := s.setPos (input.next i);
+    let curr := input.get i
+    let s    := s.setPos (input.next i)
     if curr == '\"' then
-      let s := mkNodeToken strInterpolantStrLitKind startPos c s;
+      let s := mkNodeToken strInterpolantStrLitKind startPos c s
       s.mkNode strInterpolantKind stackSize
     else if curr == '\\' then
       andthenFn (quotedCharCoreFn isQuotableCharForStrInterpolant) (parse startPos) c s
     else if curr == '{' then
-      let s := mkNodeToken strInterpolantStrLitKind startPos c s;
-      let s := p c s;
+      let s := mkNodeToken strInterpolantStrLitKind startPos c s
+      let s := p c s
       if s.hasError then s
       else
-        let pos := s.pos;
+        let pos := s.pos
         andthenFn (satisfyFn (· == '}') "expected '}'") (parse pos) c s
     else
-      parse startPos c s;
-let startPos := s.pos;
+      parse startPos c s
+let startPos := s.pos
 if input.atEnd startPos then
   s.mkEOIError
 else
-  let s := s.next input startPos;
+  let s := s.next input startPos
   parse startPos c s
 
 @[inline] def strInterpolantNoAntiquot (p : Parser) : Parser :=
@@ -73,24 +73,24 @@ def decodeStrInterpolantQuotedChar (s : String) (i : String.Pos) : Option (Char 
 match decodeQuotedChar s i with
 | some r => some r
 | none   =>
-  let c := s.get i;
-  let i := s.next i;
+  let c := s.get i
+  let i := s.next i
   if c == '{' then pure ('{', i)
   else none
 
 partial def decodeStrInterpolantStrLit (s : String) : Option String :=
 let rec loop (i : String.Pos) (acc : String) :=
-  let c := s.get i;
-  let i := s.next i;
+  let c := s.get i
+  let i := s.next i
   if c == '\"' || c == '{' then
     pure acc
   else if s.atEnd i then
     none
   else if c == '\\' then do
-    let (c, i) ← decodeStrInterpolantQuotedChar s i;
+    let (c, i) ← decodeStrInterpolantQuotedChar s i
     loop i (acc.push c)
   else
-    loop i (acc.push c);
+    loop i (acc.push c)
 loop 1 ""
 
 partial def isStrInterpolantStrLit? (stx : Syntax) : Option String :=
@@ -102,7 +102,7 @@ def expandStrInterpolantChunks (chunks : Array Syntax) (mkAppend : Syntax → Sy
 chunks.iterateM Syntax.missing fun i elem result => do
   let elem ← match elem.isStrInterpolantStrLit? with
     | none     => mkElem elem
-    | some str => mkElem (mkStxStrLit str);
+    | some str => mkElem (mkStxStrLit str)
   -- TODO: remove `(` after we write new elabDo
   (if i.val == 0 then pure elem else mkAppend result elem)
 
@@ -122,26 +122,26 @@ Syntax.expandStrInterpolantChunks chunks (fun a b => `($a ++ $b)) (fun a => `(to
 macro_rules[Lean.Parser.Term.toString]
 | `(toString! $strInterp) => mkToString! strInterp.getArgs
 
-#eval let x := 10; toString! "hello { x + 10 } world"
+#eval let x := 10 toString! "hello { x + 10 } world"
 #eval toString! "{1+1}"
 #eval toString! "{1}+{1}"
 #eval toString! "\{{1+1}}"
 #eval toString! "a{1}"
 
 def g (x : Nat) : StateRefT Nat IO Nat := do
-modify (· + x);
+modify (· + x)
 get
 
 def ex : StateRefT Nat IO Unit := do
-IO.println $ toString! ">> hello {(←g 1)}";
-IO.println $ toString! ">> world {(←g 1)}";
+IO.println $ toString! ">> hello {(←g 1)}"
+IO.println $ toString! ">> world {(←g 1)}"
 pure ()
 
 #eval ex.run' 0
 
 -- We can safely use string interpolation in macros
 macro valueOf! x:term : term =>
-  let s := quote (toString x.prettyPrint);
+  let s := quote (toString x.prettyPrint)
   `((do { let s := $s; let r := $x; IO.println (toString! "value of ({$s}) = {r}"); pure r } : IO _))
 
 #eval let s := 10; valueOf! s+2
